src/smtencoding/FStar.SMTEncoding.EncodeTerm.fst
@@ -951,7 +951,7 @@ and encode_term (t:typ) (env:env_t) : (term         (* encoding of t, expects t 
         | Tm_constant Const_set_range_of, [(arg, _); (rng, _)] ->
             encode_term arg env
 
-        | Tm_constant (Const_reify _), _ (* (_::_::_) *) ->
+        | Tm_constant Const_reify, _ (* (_::_::_) *) ->
             let e0 = TcUtil.reify_body_with_arg env.tcenv [] head (List.hd args_e) in
             if Env.debug env.tcenv <| Options.Other "SMTEncodingReify"
             then BU.print1 "Result of normalization %s\n" (Print.term_to_string e0);
