src/syntax/FStar.Syntax.Util.fst
@@ -1720,7 +1720,7 @@ let action_as_lb eff_lid a pos =
 
 (* Some reification utilities *)
 let mk_reify t =
-    let reify_ = mk (Tm_constant (FStar.Const.Const_reify None)) t.pos in
+    let reify_ = mk (Tm_constant FStar.Const.Const_reify) t.pos in
     mk (Tm_app(reify_, [as_arg t])) t.pos
 
 let mk_reflect t =
